format-version: 1.2
ontology: oba/imports/po_import

[Term]
id: PO:0000003
name: whole plant
def: "A plant structure (PO:0005679) which is a whole organism." []
synonym: "bush" NARROW []
synonym: "clonal colony" RELATED []
synonym: "colony" RELATED []
synonym: "frutex" NARROW []
synonym: "frutices" NARROW []
synonym: "gametophyte" NARROW []
synonym: "genet" BROAD []
synonym: "herb" NARROW []
synonym: "liana" NARROW []
synonym: "planta entera (Spanish)" EXACT []
synonym: "prothalli" NARROW []
synonym: "prothallium" NARROW []
synonym: "prothallus" NARROW []
synonym: "ramet" BROAD []
synonym: "seedling" NARROW []
synonym: "shrub" NARROW []
synonym: "sporophyte" NARROW []
synonym: "suffrutex" NARROW []
synonym: "suffrutices" NARROW []
synonym: "tree" NARROW []
synonym: "vine" NARROW []
synonym: "woody clump" NARROW []
synonym: "植物体全体 (Japanese)" EXACT []
is_a: PO:0009011 ! plant structure

[Term]
id: PO:0000015
name: cotyledon primordium
def: "A phyllome primordium (PO:0025128) that develops from a cotyledon anlagen (PO:0025432) and is part of a vegetative shoot apex (PO:0025223) and is committed to the development of a cotyledon (PO:0020030)." []
synonym: "cotyledon primordia" EXACT []
synonym: "portion of cotyledon primordium tissue" EXACT []
synonym: "primordio de cotiled&#243n (Spanish)" EXACT []
synonym: "子葉原基（可視的） (Japanese)" EXACT []
is_a: PO:0025128 ! phyllome primordium
relationship: BFO:0000050 PO:0025223 ! part_of vegetative shoot apex
relationship: RO:0002202 PO:0025432 ! develops_from cotyledon anlagen

[Term]
id: PO:0000017
name: vascular leaf primordium
def: "A phyllome primordium (PO:0025128) that develops from a vascular leaf anlagen (PO:0025431) and is part of a vegetative shoot apex (PO:0025223) and is committed to the development of a vascular leaf (PO:0009025)." []
synonym: "leaf primordium" EXACT []
synonym: "portion of vascular leaf primordium tissue" EXACT []
synonym: "primordio de hoja (Spanish)" EXACT []
synonym: "vascular leaf primordia" EXACT []
synonym: "葉原基 (Japanese)" EXACT []
is_a: PO:0025128 ! phyllome primordium
relationship: BFO:0000050 PO:0025223 ! part_of vegetative shoot apex
relationship: RO:0002202 PO:0025431 ! develops_from vascular leaf anlagen

[Term]
id: PO:0000034
name: vascular system
def: "A maximal portion of vascular tissue (PO:0009015) in a whole plant (PO:0000003), collective plant structure (PO:0025497), multi-tissue plant structure (PO:0025496), or cardinal part of multi-tissue plant structure (PO:0025498)." []
synonym: "sistema vascular (Spanish)" EXACT []
synonym: "vasculature" EXACT []
synonym: "維管束系 (Japanese)" EXACT []
is_a: PO:0009007 ! portion of plant tissue
disjoint_from: PO:0009002 ! plant cell
disjoint_from: PO:0009008 ! plant organ
disjoint_from: PO:0025001 ! cardinal organ part
disjoint_from: PO:0025007 ! collective plant organ structure
relationship: BFO:0000050 PO:0000003 ! part_of whole plant

[Term]
id: PO:0000037
name: shoot apex
def: "A shoot axis (PO:0025029) that is the most distal part of a shoot system (PO:0009006) and has as parts a shoot apical meristem (PO:0020148) and the youngest primordia (PO:0025127)." []
synonym: "&#225pice del epiblasto (epiblastema) (Spanish)" EXACT []
synonym: "シュート頂、茎頂 (Japanese)" EXACT []
is_a: PO:0025029 ! shoot axis

[Term]
id: PO:0000225
name: peripheral zone
def: "A portion of meristem tissue (PO:0009013) which is the organogenic region of the meristem, characterized by higher rates of cell division." []
synonym: "peripheral meristem" RELATED []
synonym: "zona perif&#233rica (Spanish)" EXACT []
synonym: "周辺帯 (Japanese)" EXACT []
is_a: PO:0009013 ! portion of meristem tissue
relationship: BFO:0000050 PO:0020148 ! part_of shoot apical meristem

[Term]
id: PO:0004010
name: meristematic cell
def: "A native plant cell (PO:0025606) synthesizing protoplasm and producing new cells by division and with only a primary cell wall." []
synonym: "c&#233lula meristem&#225tica (Spanish)" EXACT []
synonym: "stem cell" EXACT []
synonym: "分裂組織細胞 (Japanese)" EXACT []
is_a: PO:0025606 ! native plant cell

[Term]
id: PO:0004708
name: scutellar node
def: "A stem node that is the part of an embryo axis directly above the radicle where the scutellum is attached." []
synonym: "nodo escutelar (Spanish)" EXACT []
synonym: "胚盤節 (Japanese)" EXACT []
is_a: PO:0020141 ! stem node
is_a: PO:0025099 ! embryo plant structure
relationship: BFO:0000050 PO:0019018 ! part_of plant embryo axis

[Term]
id: PO:0005004
name: shoot axis node
def: "A cardinal organ part (PO:0025001) of a shoot axis (PO:0025029) where a bud (PO:0000055) may form and develop into a branch (PO:0025073), leaf (PO:0025034), flower (PO:0004541), inflorescence (PO:0009049) or nodal root (PO:0003005)." []
synonym: "nodo del epiblasto (epiblastema) (Spanish)" EXACT []
synonym: "シュート 節 (Japanese)" EXACT []
is_a: PO:0025001 ! cardinal organ part
relationship: BFO:0000050 PO:0025029 ! part_of shoot axis

[Term]
id: PO:0005352
name: xylem
def: "A portion of vascular tissue (PO:0009015) that has as part one or more tracheary elements (PO:0000290)." []
synonym: "portion of xylem tissue" EXACT []
synonym: "xilema (Spanish)" EXACT []
synonym: "木質部 (Japanese)" EXACT []
is_a: PO:0009015 ! portion of vascular tissue

[Term]
id: PO:0005597
name: cambium
def: "A lateral meristem (PO:0020145) that has as part a single layer of cambial initial cells (PO:0000295) and their derivatives, arranged orderly in radial files." []
synonym: "cambium (Spanish)" EXACT []
synonym: "形成層 (Japanese)" EXACT []
is_a: PO:0020145 ! lateral meristem

[Term]
id: PO:0005598
name: vascular cambium
def: "A cambium (PO:0005597) that is located between and gives rise to secondary xylem (PO:0005848) and secondary phloem (PO:0005043)." []
synonym: "cambium vascular (Spanish)" EXACT []
synonym: "維管束形成層 (Japanese)" EXACT []
is_a: PO:0005597 ! cambium

[Term]
id: PO:0005848
name: secondary xylem
def: "A portion of xylem (PO:0005352) tissue that develops from a vascular cambium (PO:0005598)." []
synonym: "portion of secondary xylem tissue" EXACT []
synonym: "wood" EXACT []
synonym: "xilema secundario (Spanish)" EXACT []
synonym: "二次木部 (Japanese)" EXACT []
is_a: PO:0005352 ! xylem
is_a: PO:0025409 ! secondary vascular tissue
relationship: RO:0002202 PO:0005598 ! develops_from vascular cambium

[Term]
id: PO:0006001
name: phyllome
def: "A lateral plant organ (PO:0009008) produced by a shoot apical meristem (PO:0020148)." []
synonym: "filoma (Spanish)" EXACT []
synonym: "フィロム、葉(的）器官 (Japanese)" EXACT []
is_a: PO:0009008 ! plant organ
relationship: BFO:0000050 PO:0009006 ! part_of shoot system
relationship: RO:0002202 PO:0025128 ! develops_from phyllome primordium

[Term]
id: PO:0006079
name: shoot system meristem
def: "A portion of meristem tissue (PO:0009013) that is part of a shoot system (PO:0009006)." []
synonym: "meristema del epiblasto (epiblastema) (Spanish)" EXACT []
synonym: "シュート分裂組織 (Japanese)" EXACT []
is_a: PO:0009013 ! portion of meristem tissue
relationship: BFO:0000050 PO:0009006 ! part_of shoot system

[Term]
id: PO:0006210
name: protoderm
def: "A portion of meristem tissue (PO:0009013) that is the outer layer of an apical meristem (PO:0020144), or the outer layer of a plant embryo proper (PO:0000001), and gives rise to a portion of epidermis (PO:0005679)." []
synonym: "dermatogen cell" RELATED []
synonym: "portion of protoderm tissue" EXACT []
synonym: "protodermis (Spanish)" EXACT []
synonym: "前表皮、原表皮 (Japanese)" EXACT []
is_a: PO:0009013 ! portion of meristem tissue

[Term]
id: PO:0008016
name: vegetative shoot apical meristem
def: "A shoot apical meristem (PO:0020148) that gives rise to the apical growth of vegetative tissues and organs." []
synonym: "meristema vegetativo apical del epiblasto (epiblastema) (Spanish)" EXACT []
synonym: "vegetative meristem" RELATED []
synonym: "栄養シュート頂端分裂組織 (Japanese)" EXACT []
is_a: PO:0020148 ! shoot apical meristem

[Term]
id: PO:0009002
name: plant cell
def: "A cell which is a plant structure (PO:0009011)." []
synonym: "c&#233lula vegetal (Spanish)" EXACT []
synonym: "cell" BROAD []
synonym: "植物細胞 (Japanese)" EXACT []
is_a: PO:0009011 ! plant structure
disjoint_from: PO:0009007 ! portion of plant tissue
disjoint_from: PO:0009008 ! plant organ
disjoint_from: PO:0025001 ! cardinal organ part
disjoint_from: PO:0025007 ! collective plant organ structure

[Term]
id: PO:0009006
name: shoot system
def: "A collective plant organ structure (PO:0025007) that produces shoot-borne portions of meristem tissue (PO:0009013) and the plant structures (PO:0009011) that arise from them." []
synonym: "Poaceae crown" RELATED []
synonym: "shoot" RELATED []
synonym: "sistema de epiblasto (epiblastema) (Spanish)" EXACT []
synonym: "thalli" RELATED []
synonym: "thallus" RELATED []
synonym: "tree crown" NARROW []
synonym: "シュート系、苗条系 (Japanese)" EXACT []
is_a: PO:0025007 ! collective plant organ structure

[Term]
id: PO:0009007
name: portion of plant tissue
def: "A plant structure (PO:0009011) that consists predominantly of similarly specialized plant cells (PO:0009002) of one or more types." []
synonym: "plant tissue" RELATED []
synonym: "porci&#243n de un tejido vegetal (Spanish)" EXACT []
synonym: "portion of tissue" BROAD []
synonym: "tissue" BROAD []
synonym: "植物組織の一部 (Japanese)" EXACT []
is_a: PO:0009011 ! plant structure
disjoint_from: PO:0009008 ! plant organ
disjoint_from: PO:0025001 ! cardinal organ part
disjoint_from: PO:0025007 ! collective plant organ structure

[Term]
id: PO:0009008
name: plant organ
def: "A multi-tissue plant structure (PO:0025496) that is a functional unit, is a proper part of a whole plant (PO:0000003), and includes portions of plant tissue (PO:0009007) of at least two different types that derive from a common developmental path." []
synonym: "&#243rgano vegetal (Spanish)" EXACT []
synonym: "compound plant organ" RELATED []
synonym: "organ" BROAD []
synonym: "simple plant organ" RELATED []
synonym: "植物 器官 (Japanese)" EXACT []
is_a: PO:0025496 ! multi-tissue plant structure

[Term]
id: PO:0009009
name: plant embryo
def: "A whole plant (PO:0000003) that participates in the plant embryo stage (PO:0007631)." []
synonym: "embri&#243n (Spanish)" EXACT []
synonym: "embryo" BROAD []
synonym: "germ" RELATED []
synonym: "植物胚 (Japanese)" EXACT []
is_a: PO:0000003 ! whole plant

[Term]
id: PO:0009011
name: plant structure
def: "An anatomical structure that is or was part of a plant, or was derived from a part of a plant." []
synonym: "estructura vegetal (Spanish)" EXACT []
synonym: "植物 構造 (Japanese)" EXACT []
is_a: PO:0025131 ! plant anatomical entity

[Term]
id: PO:0009013
name: portion of meristem tissue
def: "A portion of plant tissue (PO:0009007) in which plant cells (PO:0009002) have retained their embryonic characteristics, or have reverted to them secondarily, and that divide to produce new cells that can undergo differentiation to form mature tissues, i.e. they have a capacity for morphogenesis and growth." []
synonym: "meristem" EXACT []
synonym: "meristema (Spanish)" EXACT []
synonym: "meristematic tissue" EXACT []
synonym: "分裂組織 (Japanese)" EXACT []
is_a: PO:0009007 ! portion of plant tissue
relationship: BFO:0000051 PO:0004010 ! has_part meristematic cell

[Term]
id: PO:0009015
name: portion of vascular tissue
def: "A portion of plant tissue (PO:0009007) that has as part one or more tracheary elements (PO:0000290) or sieve elements (PO:0025406)." []
synonym: "porci&#243n de tejido vascular (Spanish)" EXACT []
synonym: "vascular system" RELATED []
synonym: "vascular tissue" EXACT []
synonym: "維管束細胞の一部 (Japanese)" EXACT []
is_a: PO:0009007 ! portion of plant tissue
relationship: BFO:0000050 PO:0000034 ! part_of vascular system

[Term]
id: PO:0009025
name: vascular leaf
def: "A leaf (PO:0025034) in a vascular plant." []
synonym: "ascidia" NARROW []
synonym: "ascidium" NARROW []
synonym: "crozier" RELATED []
synonym: "fiddlehead" NARROW []
synonym: "foliage leaf" EXACT []
synonym: "frond" NARROW []
synonym: "hoja vascular (Spanish)" EXACT []
synonym: "leaf, vascular" EXACT []
synonym: "macrophyll" RELATED []
synonym: "megaphyll" RELATED []
synonym: "needle-like leaf" NARROW []
synonym: "pitcher" NARROW []
synonym: "pitcher blade" NARROW []
synonym: "pitcher-blade" NARROW []
synonym: "scale-like leaf" NARROW []
synonym: "sterile frond" NARROW []
synonym: "trophophyll" NARROW []
synonym: "vascular leaves" EXACT []
synonym: "維管束のある葉, または維管束植物の葉 (Japanese)" EXACT []
is_a: PO:0025034 ! leaf
relationship: RO:0002202 PO:0000017 ! develops_from vascular leaf primordium

[Term]
id: PO:0009047
name: stem
def: "A shoot axis (PO:0025029) that is the primary axis of a plant." []
synonym: "bole" NARROW []
synonym: "ca&#241a (Spanish)" EXACT []
synonym: "cane" NARROW []
synonym: "caudex" NARROW []
synonym: "caudices" NARROW []
synonym: "culm" EXACT []
synonym: "eje primario (Spanish)" EXACT []
synonym: "primary axis" EXACT []
synonym: "primary stem" EXACT []
synonym: "primocane" NARROW []
synonym: "scape" NARROW []
synonym: "stalk" NARROW []
synonym: "tallo (Spanish)" EXACT []
synonym: "tronco (Spanish)" EXACT []
synonym: "trunk" NARROW []
synonym: "茎 (Japanese)" EXACT []
is_a: PO:0025029 ! shoot axis

[Term]
id: PO:0019018
name: plant embryo axis
def: "A plant axis (PO:0025004) that is the axial part of a plant embryo (PO:0009009)." []
synonym: "eje del embri&#243n (Spanish)" EXACT []
synonym: "embryo axis" BROAD []
synonym: "hypocotyl-root axis" EXACT []
synonym: "zygotic plant embryo axis" NARROW []
synonym: "植物胚軸 (Japanese)" EXACT []
is_a: PO:0025004 ! plant axis
is_a: PO:0025099 ! embryo plant structure
relationship: BFO:0000050 PO:0009009 ! part_of plant embryo

[Term]
id: PO:0020030
name: cotyledon
def: "A vascular leaf (PO:0009025) formed at the first shoot node (PO:0005004) of a plant embryo (PO:0009009) or a seedling (PO:0000003)." []
synonym: "cotiled&#243n (Spanish)" EXACT []
synonym: "seed leaf" EXACT []
synonym: "子葉 (Japanese)" EXACT []
is_a: PO:0009025 ! vascular leaf
relationship: RO:0002202 PO:0000015 ! develops_from cotyledon primordium

[Term]
id: PO:0020141
name: stem node
def: "A shoot node that is part of a stem." []
synonym: "nodo del tallo (Spanish)" EXACT []
synonym: "茎節 (Japanese)" EXACT []
is_a: PO:0005004 ! shoot axis node
relationship: BFO:0000050 PO:0009047 ! part_of stem

[Term]
id: PO:0020144
name: apical meristem
def: "A maximal portion of meristem tissue (PO:0009013) located at a shoot apex (PO:0000037) or root tip (PO:0000025)." []
synonym: "AM" EXACT []
synonym: "meristema apical (Spanish)" EXACT []
synonym: "primary meristem" RELATED []
synonym: "promeristem" BROAD []
synonym: "頂端分裂組織 (Japanese)" EXACT []
is_a: PO:0009013 ! portion of meristem tissue
relationship: BFO:0000051 PO:0006210 ! has_part protoderm

[Term]
id: PO:0020145
name: lateral meristem
def: "A portion of meristem (PO:0009013) tissue located parallel to the sides of a shoot axis (PO:0025029) or root (PO:0009005) that participates in lateral growth." []
synonym: "lateral growth meristem" EXACT []
synonym: "meristema lateral (Spanish)" EXACT []
synonym: "secondary meristem" RELATED []
synonym: "側 分裂組織 (Japanese)" EXACT []
is_a: PO:0009013 ! portion of meristem tissue
relationship: BFO:0000050 PO:0025004 ! part_of plant axis

[Term]
id: PO:0020148
name: shoot apical meristem
def: "A shoot system meristem (PO:0006079) formed at the apex of the shoot axis (PO:0025029), including those originating from an axillary bud meristem (PO:0000232)." []
synonym: "meristema apical del epiblasto (epiblastema) (Spanish)" EXACT []
synonym: "primary shoot meristem" RELATED []
synonym: "promeristem" BROAD []
synonym: "SAM" EXACT []
synonym: "茎頂分裂組織 (Japanese)" EXACT []
is_a: PO:0006079 ! shoot system meristem
is_a: PO:0020144 ! apical meristem
relationship: BFO:0000050 PO:0000037 ! part_of shoot apex

[Term]
id: PO:0025001
name: cardinal organ part
def: "A cardinal part of multi-tissue plant structure (PO:0025498) that is a proper part of a plant organ (PO:0009008) and includes portions of plant tissue (PO:0009007) of at least two different types." []
synonym: "cardinal part of plant organ" EXACT []
synonym: "parte de un &#243rgano cardinal (Spanish)" EXACT []
synonym: "基本的な（主要な）器官部 (Japanese)" EXACT []
is_a: PO:0025498 ! cardinal part of multi-tissue plant structure
intersection_of: PO:0025498 ! cardinal part of multi-tissue plant structure
intersection_of: BFO:0000050 PO:0009008 ! part_of plant organ
relationship: BFO:0000050 PO:0009008 ! part_of plant organ

[Term]
id: PO:0025004
name: plant axis
def: "An axial plant organ (PO:0009008)." []
synonym: "eje de la planta (Spanish)" EXACT []
synonym: "plant axes" EXACT []
synonym: "植物軸（軸柱） (Japanese)" EXACT []
is_a: PO:0009008 ! plant organ

[Term]
id: PO:0025007
name: collective plant organ structure
def: "A collective plant structure (PO:0025497) that is a proper part of a whole plant (PO:0000003), and is composed of two or more adjacent plant organs (PO:0009008) and the associated portions of plant tissue (PO:0009007)." []
synonym: "estructura vegetal colectiva de &#243rgano (Spanish)" EXACT []
synonym: "集合植物器官構造 (Japanese)" EXACT []
is_a: PO:0025497 ! collective plant structure
relationship: BFO:0000051 PO:0009008 ! has_part plant organ

[Term]
id: PO:0025028
name: embryo plant cell
def: "A native plant cell (PO:0025606) that is part of a plant embryo (PO:0009009)." []
synonym: "c&#233lula embri&#243nica vegetal (Spanish)" EXACT []
synonym: "embryo cell" BROAD []
synonym: "embryonic cell" BROAD []
synonym: "embryonic plant cell" EXACT []
synonym: "胚性植物細胞 (Japanese)" EXACT []
is_a: PO:0025099 ! embryo plant structure
is_a: PO:0025606 ! native plant cell
intersection_of: PO:0025606 ! native plant cell
intersection_of: BFO:0000050 PO:0009009 ! part_of plant embryo
relationship: BFO:0000050 PO:0009009 ! part_of plant embryo

[Term]
id: PO:0025029
name: shoot axis
def: "A plant axis (PO:0025004) that is part of a shoot system (PO:0009006)." []
synonym: "caullome" EXACT []
synonym: "eje del epiblasto (epiblastema) (Spanish)" EXACT []
synonym: "shoot" RELATED []
synonym: "シュート軸 (Japanese)" EXACT []
is_a: PO:0025004 ! plant axis
relationship: BFO:0000050 PO:0009006 ! part_of shoot system

[Term]
id: PO:0025034
name: leaf
def: "A phyllome (PO:0006001) that is not associated with a reproductive structure." []
synonym: "hoja (Spanish)" EXACT []
synonym: "葉 (Japanese)" EXACT []
is_a: PO:0006001 ! phyllome

[Term]
id: PO:0025099
name: embryo plant structure
def: "A plant structure (PO:0009011) that is part of an plant embryo (PO:0009009)." []
synonym: "embryonic plant structure" EXACT []
synonym: "estructura vegetal embri&#243nica (Spanish)" EXACT []
synonym: "胚性植物構造 (Japanese)" EXACT []
is_a: PO:0009011 ! plant structure
intersection_of: PO:0009011 ! plant structure
intersection_of: BFO:0000050 PO:0009009 ! part_of plant embryo
relationship: BFO:0000050 PO:0009009 ! part_of plant embryo

[Term]
id: PO:0025127
name: primordium
def: "A portion of meristem tissue (PO:0009013) that has as parts protoderm (PO:0006210) and sub-epidermal meristematic tissue and is committed to the development of a particular plant structure (PO:0009011)." []
synonym: "portion of primordial tissue" EXACT []
synonym: "portion of primordium tissue" EXACT []
synonym: "primordia" EXACT []
synonym: "primordio (Spanish)" EXACT []
synonym: "原基（可視的）  (Japanese)" EXACT []
is_a: PO:0009013 ! portion of meristem tissue

[Term]
id: PO:0025128
name: phyllome primordium
def: "A primordium (PO:0025127) that develops from a phyllome anlagen (PO:0025430) and is part of a shoot apex (PO:0000037) and is committed to the development of a phyllome (PO:0006001)." []
synonym: "phyllome primordia" EXACT []
synonym: "portion of phyllome primordium tissue" EXACT []
synonym: "primordio del filoma (Spanish)" EXACT []
synonym: "フィロム原基（可視的）  (Japanese)" EXACT []
is_a: PO:0025127 ! primordium
relationship: BFO:0000050 PO:0000037 ! part_of shoot apex
relationship: RO:0002202 PO:0025430 ! develops_from phyllome anlagen

[Term]
id: PO:0025131
name: plant anatomical entity
def: "An anatomical entity that is or was part of a plant." []
synonym: "entidad anat&#243mica vegetal (Spanish)" EXACT []
synonym: "植物 解剖学（形態）的実体 (Japanese)" EXACT []

[Term]
id: PO:0025223
name: vegetative shoot apex
def: "A shoot apex PO:0000037) that has as part a vegetative shoot apical meristem (PO:0008016)." []
synonym: "&#225pice vegetativo del epiblasto (epiblastema) (Spanish)" EXACT []
synonym: "栄養シュート頂、栄養枝頂 (Japanese)" EXACT []
is_a: PO:0000037 ! shoot apex
relationship: BFO:0000051 PO:0008016 ! has_part vegetative shoot apical meristem

[Term]
id: PO:0025233
name: portion of embryo plant tissue
def: "A portion of plant tissue that is part of a plant embryo." []
synonym: "portion of embryo tissue" BROAD []
synonym: "portion of embryonic plant tissue" EXACT []
synonym: "tejido embri&#243nico vegetal (Spanish)" EXACT []
synonym: "植物胚性組織 の一部   (Japanese)" EXACT []
is_a: PO:0009007 ! portion of plant tissue
is_a: PO:0025099 ! embryo plant structure
intersection_of: PO:0009007 ! portion of plant tissue
intersection_of: BFO:0000050 PO:0009009 ! part_of plant embryo
relationship: BFO:0000050 PO:0009009 ! part_of plant embryo

[Term]
id: PO:0025321
name: cotyledonary node
def: "A stem node from which one or more cotyledons grow." []
synonym: "nodo del cotiled&#243n (Spanish)" EXACT []
synonym: "子葉節 (Japanese)" EXACT []
is_a: PO:0020141 ! stem node

[Term]
id: PO:0025409
name: secondary vascular tissue
def: "A portion of vascular tissue (PO:0009015) that develops from a vascular cambium (PO:0005598)." []
synonym: "tejido vascular secundario (Spanish)" EXACT []
synonym: "二次維管組織 (Japanese)" EXACT []
is_a: PO:0009015 ! portion of vascular tissue
intersection_of: PO:0009015 ! portion of vascular tissue
intersection_of: RO:0002202 PO:0005598 ! develops_from vascular cambium
relationship: RO:0002202 PO:0005598 ! develops_from vascular cambium

[Term]
id: PO:0025430
name: phyllome anlagen
def: "A portion of meristem tissue (PO:0009013) that is part of a peripheral zone (PO:0000225) of a shoot apical meristem (PO:0020148) and will give rise to a phyllome primordium (PO:0025128)." []
synonym: "phyllome meristem" BROAD []
synonym: "フィロム原基 (Japanese)" EXACT []
is_a: PO:0009013 ! portion of meristem tissue
relationship: BFO:0000050 PO:0000225 ! part_of peripheral zone

[Term]
id: PO:0025431
name: vascular leaf anlagen
def: "A phyllome anlagen (PO:0025430) that will give rise to a vascular leaf primordium (PO:0000017) and is part of a peripheral zone (PO:0000225) of a shoot apical meristem (PO:0020148)." []
synonym: "leaf meristem" BROAD []
synonym: "維管束系葉原基 (Japanese)" EXACT []
is_a: PO:0025430 ! phyllome anlagen
relationship: BFO:0000050 PO:0008016 ! part_of vegetative shoot apical meristem

[Term]
id: PO:0025432
name: cotyledon anlagen
def: "A phyllome anlagen (PO:0025430) that will give rise to a cotyledon primordium (PO:0000015) and is part of a peripheral zone (PO:000225) of an embryo shoot apical meristem (PO:0006362)." []
synonym: "precursor de cotiled&#243n (Spanish)" EXACT []
synonym: "子葉原基 (Japanese)" EXACT []
is_a: PO:0025233 ! portion of embryo plant tissue
is_a: PO:0025430 ! phyllome anlagen
relationship: BFO:0000050 PO:0009009 ! part_of plant embryo

[Term]
id: PO:0025496
name: multi-tissue plant structure
def: "A plant structure (PO:0009011) that has as parts two or more portions of plant tissue (PO:0009007) of at least two different types and which through specific morphogenetic processes forms a single structural unit demarcated by primarily bona-fide boundaries from other structural units of different types." []
synonym: "estructura vegetal con m&#250ltiples tejidos (Spanish)" EXACT []
synonym: "複数の組織からなる植物構造 (Japanese)" EXACT []
is_a: PO:0009011 ! plant structure

[Term]
id: PO:0025497
name: collective plant structure
def: "A plant structure (PO:0009011) that is a proper part of a whole plant (PO:0000003) and includes two or more adjacent plant organs (PO:0009008) or adjacent cardinal organ parts (PO:0025001), along with any associated portions of plant tissue (PO:0009007)." []
synonym: "estructura vegetal colectiva (Spanish)" EXACT []
synonym: "集合的植物構造 (Japanese)" EXACT []
is_a: PO:0009011 ! plant structure

[Term]
id: PO:0025498
name: cardinal part of multi-tissue plant structure
def: "A plant structure (PO:0009011) that is a proper part of a multi-tissue plant structure (PO:0025496) and includes portions of plant tissues (PO:0009007) of at least two different types." []
synonym: "parte cardinal de estructura vegetal con m&#250ltiples tejidos (Spanish)" EXACT []
synonym: "複数の組織からなる植物構造の基本（主要）部分 (Japanese)" EXACT []
is_a: PO:0009011 ! plant structure
relationship: BFO:0000050 PO:0025496 ! part_of multi-tissue plant structure

[Term]
id: PO:0025606
name: native plant cell
def: "A plant cell (PO:0009002) that is either part of a multicellular whole plant (PO:0000003) 'in vivo' or a unicellular organism 'in natura' (i.e. part of a natural environment)." []
is_a: PO:0009002 ! plant cell

[Typedef]
id: BFO:0000050
name: part_of
is_transitive: true

[Typedef]
id: BFO:0000051
name: has_part
is_transitive: true

[Typedef]
id: RO:0002202
name: develops_from
is_transitive: true

